Axioms.fst
@@ -1,0 +1,40 @@
+module Axioms
+
+(** Whole bunch of axioms that we use throughout the rest of the proofs *)
+
+open Spec.Lib.IntTypes
+open Spec.Lib.IntSeq
+
+(** Axiom: Two sequences are equal iff all their elements are equal *)
+val intseq_eq: t:inttype -> len:size_t ->
+  Lemma (forall (a:intseq t len) (b:intseq t len).
+                                   (a == b) <==> (forall x. a.[x] == b.[x]))
+    [SMTPat (intseq t len)]
+let intseq_eq t len = admit ()
+
+(** Axiom: Subsequence actually gives us the subsequence *)
+val sub_semantics:
+  #t:inttype ->
+  #len:size_t ->
+  s:intseq t len ->
+  start:size_t ->
+  n:size_t{start + n <= len} ->
+  Lemma (forall (x:size_t{x < n}). (sub s start n).[x] == s.[start + x])
+  //    [SMTPat (sub s start n)]
+let sub_semantics #t #len s start n = admit()
+
+(** Axiom: Two sequences are same iff their LE representation is same *)
+val eq_nat_from_intseq:
+  #t:inttype ->
+  #len:size_t ->
+  a:intseq t len ->
+  b:intseq t len ->
+  Lemma (a == b <==> nat_from_intseq_le a == nat_from_intseq_le b)
+let eq_nat_from_intseq #t #len a b = admit ()
+
+    assume
+(** Assumption: An [append] function is provided by the API *)
+val append: #len1:size_t -> #len2:size_t ->
+  #len:size_t{len=len1+len2} -> s1:lbytes len1 -> s2:lbytes len2 ->
+  s:lbytes len{(sub s 0 len1 == s1) /\
+               (sub s len1 len2 == s2)}
